update Syntax and test tlogic

src/tlogic/LogicSyntaxHOAS.v
@@ -29,11 +29,11 @@ Module Syntax.
     | persistently (p : t) : t
     | plainly (p : t) : t
     | upd (p : t) : t
-    (* for invariant system *)
-    | owni (i : positive) (p : t)
-    | syn_inv_auth_l (ps : list (prod positive t))
-    (* Non strictly positive occurrence *)
-    (* | own_inv_auth (ps : gmap positive t) *)
+    (* (* for invariant system *) *)
+    (* | owni (i : positive) (p : t) *)
+    (* | syn_inv_auth_l (ps : list (prod positive t)) *)
+    (* (* Non strictly positive occurrence *) *)
+    (* (* | own_inv_auth (ps : gmap positive t) *) *)
     .
 
   End SYNTAX.
@@ -42,12 +42,12 @@ Module Syntax.
 
     Context `{type : Type}.
     Context `{Typ : forall formula : Type, type -> Type}.
-    Context `{As : (type -> Type) -> Type}.
+    Context `{As : forall formula : Type, Type}.
 
     Fixpoint formula (n : index) : Type :=
       match n with
-      | O => @t type Typ (As (Typ Empty_set)) Empty_set
-      | S m => @t type Typ (As (Typ (formula m))) (formula m)
+      | O => @t type Typ (As Empty_set) Empty_set
+      | S m => @t type Typ (As (formula m)) (formula m)
       (* | S m => @t type Typ (As (Typ (@t type Typ (As (Typ (formula m))) (formula m)))) (formula m) *)
       end.
 
@@ -57,15 +57,17 @@ Module Syntax.
 
     Context `{type : Type}.
     Context `{Typ : forall formula : Type, type -> Type}.
-    Context `{As : (type -> Type) -> Type}.
+    Context `{As : forall formula : Type, Type}.
 
     Local Notation formulas := (@formula type Typ As).
 
     Context `{Σ : GRA.t}.
-    Context `{@PCM.GRA.inG (IInvSetRA formulas) Σ}.
+    (* Context `{@PCM.GRA.inG (IInvSetRA formulas) Σ}. *)
 
-    Context `{interp_atoms_0 : As (Typ Empty_set) -> iProp}.
-    Context `{interp_atoms : forall (n : index), As (Typ (formulas n)) -> iProp}.
+    Context `{interp_atoms_0 : As Empty_set -> iProp}.
+    Context `{interp_atoms : forall (n : index), As (formulas n) -> iProp}.
+    (* Context `{interp_atoms_0 : As (Typ Empty_set) -> iProp}. *)
+    (* Context `{interp_atoms : forall (n : index), As (Typ (formulas n)) -> iProp}. *)
 
     Fixpoint to_semantics_0 (syn : formulas O) : iProp :=
       match syn with
@@ -83,8 +85,8 @@ Module Syntax.
       | persistently p => Persistently (to_semantics_0 p)
       | plainly p => IProp.Plainly (to_semantics_0 p)
       | upd p => Upd (to_semantics_0 p)
-      | owni i p => @OwnI Σ formulas _ O i p
-      | syn_inv_auth_l ps => @inv_auth Σ formulas _ O (list_to_map ps)
+      (* | owni i p => @OwnI Σ formulas _ O i p *)
+      (* | syn_inv_auth_l ps => @inv_auth Σ formulas _ O (list_to_map ps) *)
       end.
 
     Fixpoint to_semantics n : formulas n -> iProp :=
@@ -107,8 +109,8 @@ Module Syntax.
         | persistently p => Persistently (to_semantics_aux p)
         | plainly p => IProp.Plainly (to_semantics_aux p)
         | upd p => Upd (to_semantics_aux p)
-        | owni i p => @OwnI Σ formulas _ (S m) i p
-        | syn_inv_auth_l ps => @inv_auth Σ formulas _ (S m) (list_to_map ps)
+        (* | owni i p => @OwnI Σ formulas _ (S m) i p *)
+        (* | syn_inv_auth_l ps => @inv_auth Σ formulas _ (S m) (list_to_map ps) *)
         end
       end.
 
@@ -118,18 +120,21 @@ Module Syntax.
 
     Context `{type : Type}.
     Context `{Typ : forall formula : Type, type -> Type}.
-    Context `{As : (type -> Type) -> Type}.
+    Context `{As : forall formula : Type, Type}.
+    (* Context `{As : (type -> Type) -> Type}. *)
 
     Local Notation formulas := (@formula type Typ As).
 
     Context `{Σ : GRA.t}.
-    Context `{@PCM.GRA.inG (IInvSetRA formulas) Σ}.
+    (* Context `{@PCM.GRA.inG (IInvSetRA formulas) Σ}. *)
 
-    Context `{interp_atoms_0 : As (Typ Empty_set) -> iProp}.
-    Context `{interp_atoms : forall (n : index), As (Typ (formulas n)) -> iProp}.
+    Context `{interp_atoms_0 : As Empty_set -> iProp}.
+    Context `{interp_atoms : forall (n : index), As (formulas n) -> iProp}.
+    (* Context `{interp_atoms_0 : As (Typ Empty_set) -> iProp}. *)
+    (* Context `{interp_atoms : forall (n : index), As (Typ (formulas n)) -> iProp}. *)
 
     Global Instance IISet : @IInvSet Σ formulas :=
-      {| prop := @to_semantics type Typ As Σ _ interp_atoms_0 interp_atoms |}.
+      {| prop := @to_semantics type Typ As Σ interp_atoms_0 interp_atoms |}.
 
   End INDEXED_INVSET.
 
@@ -137,18 +142,21 @@ Module Syntax.
 
     Context `{type : Type}.
     Context `{Typ : forall formula : Type, type -> Type}.
-    Context `{As : (type -> Type) -> Type}.
+    Context `{As : forall formula : Type, Type}.
+    (* Context `{As : (type -> Type) -> Type}. *)
 
     Local Notation formulas := (@formula type Typ As).
 
     Context `{Σ : GRA.t}.
-    Context `{@PCM.GRA.inG (IInvSetRA formulas) Σ}.
+    (* Context `{@PCM.GRA.inG (IInvSetRA formulas) Σ}. *)
 
-    Context `{interp_atoms_0 : As (Typ Empty_set) -> iProp}.
-    Context `{interp_atoms : forall (n : index), As (Typ (formulas n)) -> iProp}.
+    Context `{interp_atoms_0 : As Empty_set -> iProp}.
+    Context `{interp_atoms : forall (n : index), As (formulas n) -> iProp}.
+    (* Context `{interp_atoms_0 : As (Typ Empty_set) -> iProp}. *)
+    (* Context `{interp_atoms : forall (n : index), As (Typ (formulas n)) -> iProp}. *)
 
     Global Program Instance IIIn (i : index) (p : formulas i)
-      : @IInvIn Σ formulas (IISet (interp_atoms_0:=interp_atoms_0) (interp_atoms:=interp_atoms)) i (@to_semantics type Typ As Σ _ interp_atoms_0 interp_atoms i p) :=
+      : @IInvIn Σ formulas (IISet (interp_atoms_0:=interp_atoms_0) (interp_atoms:=interp_atoms)) i (@to_semantics type Typ As Σ interp_atoms_0 interp_atoms i p) :=
       { inhabitant := p }.
     Next Obligation.
       intros. simpl. done.
@@ -158,628 +166,510 @@ Module Syntax.
 
 End Syntax.
 
-TODO
-  (* How about not allowing atoms to refer to syntax at all? *)
 
-Section TLOGIC.
 
-  Local Notation index := nat.
 
-  Section TYPE.
 
-    Inductive type : Type :=
-    | baseT (t : Type) : type
-    | formulaT : type
-    | funT : type -> type -> type
-    | pgmapT : type -> type.
 
-  End TYPE.
 
-  Section INTERP_TYPE.
 
-    Fixpoint Typ {form : Type} (ty : type) : Type :=
-      match ty with
-      | baseT b => b
-      | formulaT => form
-      | funT ty1 ty2 => (@Typ form ty1 -> @Typ form ty2)
-      | pgmapT ty1 => gmap positive (@Typ form ty1)
-      end.
+(*   Section RED. *)
+
+(*     Context `{Σ : GRA.t}. *)
+(*     Context `{As : (type -> Type) -> Type}. *)
+(*     (* Context `{T : Type}. *) *)
+(*     (* Context `{TSem : T -> Type}. *) *)
+(*     (* Context `{As : (@type T -> Type) -> Type}. *) *)
 
-  End INTERP_TYPE.
+(*     Local Notation typing := (@Typ As). *)
+(*     Local Notation Formulas := (fun (i : index) => @t (typing i) (As (typing i))). *)
+(*     (* Local Notation typing := (@Typ T TSem As). *) *)
+(*     (* Local Notation Formulas := (fun (i : index) => @t T (typing i) (As (typing i))). *) *)
 
-  Section FORMULA.
+(*     Context `{interp_atoms : forall (n : index), As (typing n) -> iProp}. *)
 
-    Context `{A : forall formula : Type, Type}.
+(*     Local Notation Sem := (fun i p => @to_semantics Σ As interp_atoms i p). *)
+(*     (* Local Notation Sem := (fun i p => @to_semantics Σ T TSem As interp_atoms i p). *) *)
 
-    Definition Formula : index -> Type :=
-      @Syntax.formula type (@Typ) A.
+(*     Lemma to_semantics_empty *)
+(*           n *)
+(*       : *)
+(*       Sem n empty = emp%I. *)
+(*     Proof. *)
+(*       induction n; ss. *)
+(*     Qed. *)
 
-  End FORMULA.
+(*     Lemma to_semantics_red_sepconj *)
+(*           n p q *)
+(*       : *)
+(*       Sem n (sepconj p q) = ((Sem n p) ∗ (Sem n q))%I. *)
+(*     Proof. *)
+(*       induction n; ss. *)
+(*     Qed. *)
 
-  Section INTERP.
+(*     Lemma to_semantics_red_or *)
+(*           n p q *)
+(*       : *)
+(*       Sem n (or p q) = ((Sem n p) ∨ (Sem n q))%I. *)
+(*     Proof. *)
+(*       induction n; ss. *)
+(*     Qed. *)
 
-    Context `{A : forall formula : Type, Type}.
-    Context `{Σ : GRA.t}.
-    Context `{interp_atoms : forall (formula : Type), A formula -> iProp}.
+(*     Lemma to_semantics_red_atom *)
+(*           n a *)
+(*       : *)
+(*       Sem n (atom a) = interp_atoms n a. *)
+(*     Proof. *)
+(*       induction n; ss. *)
+(*     Qed. *)
 
-    Definition formula_sem : forall n, Formula n -> iProp :=
-      @Syntax.to_semantics type (@Typ) A Σ interp_atoms.
+(*     Lemma to_semantics_red_ex *)
+(*           n ty f *)
+(*       : *)
+(*       Sem n (ex ty f) = (∃ (x : typing n ty), Sem n (f x))%I. *)
+(*     Proof. *)
+(*       induction n; ss. *)
+(*     Qed. *)
 
-  End INTERP.
+(*     Lemma to_semantics_red_lift *)
+(*           n p *)
+(*       : *)
+(*       Sem (S n) (lift p) = Sem n p. *)
+(*     Proof. *)
+(*       ss. *)
+(*     Qed. *)
 
-End TLOGIC.
+(*   End RED. *)
 
-Section Atom.
+(*   Section GMAP. *)
 
-  Context `{Σ : GRA.t}.
+(*     Context `{Σ : GRA.t}. *)
+(*     Context `{As : (type -> Type) -> Type}. *)
 
-  Class Atom :=
-    { T : Type
-    ; interp : T -> iProp
-    }.
+(*     Local Notation typing := (@Typ As). *)
+(*     Local Notation Formulas := (fun (i : index) => @t (typing i) (As (typing i))). *)
 
-End Atom.
+(*     Context `{interp_atoms : forall (n : index), As (typing n) -> iProp}. *)
 
-Module Atoms.
+(*     (* Maybe we can make Syntax as an instance of bi. *) *)
+(*     Definition star_gmap *)
+(*                (n : index) (I : typing (S n) (pgmapT formulaT)) *)
+(*                (f : positive -> Formulas n -> Formulas n) *)
+(*       : Formulas n := *)
+(*       fold_right (fun hd tl => @sepconj (typing n) (As (typing n)) (uncurry f hd) tl) empty (map_to_list I). *)
+
 
-  Section ATOMS.
+(*     Local Notation Sem := (fun i p => @to_semantics Σ As interp_atoms i p). *)
 
-    Context `{Σ : GRA.t}.
-
-    Inductive t {form : Type} : Type :=
-    | own {A : Atom} (a : A.(T))
-    | owni (i : positive) (p : form)
-    | syn_inv_auth_l (ps : list (prod positive form))
-    .
-
-  End ATOMS.
-
-  Section INTERP.
-
-    Context `{Σ : PCM.GRA.t}.
-
-    Local Notation Formulas := (@Formula (@t Σ)).
-
-    Context `{@PCM.GRA.inG (IInvSetRA Formulas) Σ}.
-    (* Context `{@PCM.GRA.inG (PCM.URA.pointwise index PCM.CoPset.t) Σ}. *)
-    (* Context `{@PCM.GRA.inG (PCM.URA.pointwise index PCM.Gset.t) Σ}. *)
-
-    Definition to_semantics {form : Type} (a : @t Σ form) : iProp :=
-      match a with
-      | @own _ _ A r => A.(interp) r
-      | owni i p => @OwnI Σ Formulas _ n i p
-      | syn_inv_auth_l ps => @inv_auth Σ Formulas _ n (list_to_map ps)
-      end.
-    Context `{interp_atoms : forall (formula : Type), A formula -> iProp}.
-
-  End INTERP.
-
-End Atoms.
-
-Section TL.
-
-  Context `{Σ : PCM.GRA.t}.
-
-  Local Notation Formulas := (@Formula (@Atoms.t Σ)).
-
-  Context `{@PCM.GRA.inG (IInvSetRA Formulas) Σ}.
-  (* Context `{@PCM.GRA.inG (PCM.URA.pointwise index PCM.CoPset.t) Σ}. *)
-  (* Context `{@PCM.GRA.inG (PCM.URA.pointwise index PCM.Gset.t) Σ}. *)
-
-  Local Notation AtomSem := (@Atoms.to_semantics Σ _).
-  (* Local Notation AtomSem := (@Atoms.to_semantics Σ _ _ _). *)
-  Local Notation SynSem := (@formula_sem (@Atoms.t Σ) Σ AtomSem).
-
-  Global Instance SynIISet : @IInvSet Σ Formulas := (@Syntax.IISet Σ (@Atoms.t Σ) AtomSem).
-
-
-
-
-End TL.
-
-
-
-
-
-
-
-  Section RED.
-
-    Context `{Σ : GRA.t}.
-    Context `{As : (type -> Type) -> Type}.
-    (* Context `{T : Type}. *)
-    (* Context `{TSem : T -> Type}. *)
-    (* Context `{As : (@type T -> Type) -> Type}. *)
-
-    Local Notation typing := (@Typ As).
-    Local Notation Formulas := (fun (i : index) => @t (typing i) (As (typing i))).
-    (* Local Notation typing := (@Typ T TSem As). *)
-    (* Local Notation Formulas := (fun (i : index) => @t T (typing i) (As (typing i))). *)
-
-    Context `{interp_atoms : forall (n : index), As (typing n) -> iProp}.
-
-    Local Notation Sem := (fun i p => @to_semantics Σ As interp_atoms i p).
-    (* Local Notation Sem := (fun i p => @to_semantics Σ T TSem As interp_atoms i p). *)
-
-    Lemma to_semantics_empty
-          n
-      :
-      Sem n empty = emp%I.
-    Proof.
-      induction n; ss.
-    Qed.
-
-    Lemma to_semantics_red_sepconj
-          n p q
-      :
-      Sem n (sepconj p q) = ((Sem n p) ∗ (Sem n q))%I.
-    Proof.
-      induction n; ss.
-    Qed.
-
-    Lemma to_semantics_red_or
-          n p q
-      :
-      Sem n (or p q) = ((Sem n p) ∨ (Sem n q))%I.
-    Proof.
-      induction n; ss.
-    Qed.
-
-    Lemma to_semantics_red_atom
-          n a
-      :
-      Sem n (atom a) = interp_atoms n a.
-    Proof.
-      induction n; ss.
-    Qed.
-
-    Lemma to_semantics_red_ex
-          n ty f
-      :
-      Sem n (ex ty f) = (∃ (x : typing n ty), Sem n (f x))%I.
-    Proof.
-      induction n; ss.
-    Qed.
-
-    Lemma to_semantics_red_lift
-          n p
-      :
-      Sem (S n) (lift p) = Sem n p.
-    Proof.
-      ss.
-    Qed.
-
-  End RED.
-
-  Section GMAP.
-
-    Context `{Σ : GRA.t}.
-    Context `{As : (type -> Type) -> Type}.
-
-    Local Notation typing := (@Typ As).
-    Local Notation Formulas := (fun (i : index) => @t (typing i) (As (typing i))).
-
-    Context `{interp_atoms : forall (n : index), As (typing n) -> iProp}.
-
-    (* Maybe we can make Syntax as an instance of bi. *)
-    Definition star_gmap
-               (n : index) (I : typing (S n) (pgmapT formulaT))
-               (f : positive -> Formulas n -> Formulas n)
-      : Formulas n :=
-      fold_right (fun hd tl => @sepconj (typing n) (As (typing n)) (uncurry f hd) tl) empty (map_to_list I).
-
-
-    Local Notation Sem := (fun i p => @to_semantics Σ As interp_atoms i p).
-
-    Lemma star_gmap_iProp
-          n I f
-      :
-      Sem n (star_gmap n I f) =
-        ([∗ map] i ↦ p ∈ I, Sem n (f i p))%I.
-    Proof.
-      ss. unfold big_opM. rewrite seal_eq. unfold big_op.big_opM_def.
-      unfold star_gmap. ss. remember (map_to_list I) as L.
-      clear HeqL I. induction L.
-      { ss. apply to_semantics_empty. }
-      ss. rewrite to_semantics_red_sepconj. rewrite IHL. f_equal.
-      destruct a. ss.
-    Qed.
-
-  End GMAP.
-
-
-
-
-
-
-
-
-
-
-(* Old version *)
-Module Syntax.
-
-  Local Notation index := nat.
-
-  Section TYPE.
-
-    (* Context `{T : Type}. *)
-
-    Inductive type : Type :=
-    | baseT (t : Type) : type
-    (* | baseT (t : T) : type *)
-    | formulaT : type
-    (* | prodT : type -> type -> type *)
-    (* | sumT : type -> type -> type *)
-    (* | listT : type -> type *)
-    | funT : type -> type -> type
-    (* | positiveT : type *)
-    | pgmapT : type -> type.
-    (* | gmapT (K : Type) {EqDec : EqDecision K} {Cnt : Countable K} : type -> type. *)
-
-  (* If we define for a general gmapT with EqDec and Countable,
-      universe inconsistency when checking (in TemporalLogic.Atoms)
-      ==========
-      Context `{Σ : GRA.t}.
-      Context `{T : Type}.
-      Context `{TSem : T -> Type}.
-      Local Notation typing := (@Syntax.Typ T TSem (@t T)).
-      Local Notation As := (fun (i : index) => @t T (typing i)).
-
-      Context `{@GRA.inG (IInvSetRA As) Σ}.
-      ==========
-      with an error message
-      ==========
-      The term "t" has type
-      "Type@{max(Set+1,Fairness.LogicSyntaxHOAS.59,Syntax.type.u0+1,Fairness.LogicSyntaxHOAS.64,Fairness.LogicSyntaxHOAS.65,RelDecision.u0,RelDecision.u1)}"
-      while it is expected to have type "Type@{IInvSetRA.u0}" (universe inconsistency: Cannot enforce
-      Fairness.LogicSyntaxHOAS.64 <= IInvSetRA.u0 because IInvSetRA.u0 <= InvSetRA.u0
-      <= URA.agree_obligation_4.u0 <= URA.t.u0 < MRet.u0 = Fairness.LogicSyntaxHOAS.64).
-      ==========
-      Seems like there is a strict order between URA.t and MRet,
-      and either EqDec or Countable uses MRet.
-      ==========
-      Found out that PCM.GRA.of_list introduces URA.t.u0 = RA.t.u0 < MRet.u0.
-   *)
-
-  End TYPE.
-
-  Section SYNTAX.
-
-    (* Context `{T : Type}. *)
-    Context `{Typ : type -> Type}.
-    (* Context `{Typ : @type T -> Type}. *)
-    Context `{A : Type}.
-
-    Inductive t : Type :=
-      atom (a : A) : t
-    | lift : (Typ formulaT) -> t
-    | sepconj (p q : t) : t
-    | pure (P : Prop) : t
-    | univ : forall ty, (Typ ty -> t) -> t
-    | ex : forall ty, (Typ ty -> t) -> t
-    | and (p q : t) : t
-    | or (p q : t) : t
-    | impl (p q : t) : t
-    | wand (p q : t) : t
-    | empty : t
-    | persistently (p : t) : t
-    | plainly (p : t) : t
-    | upd (p : t) : t
-    .
-
-  End SYNTAX.
-
-  Section INTERP_TYPE.
-
-    (* Context `{T : Type}. *)
-    (* Context `{TSem : T -> Type}. *)
-    Context `{As : (type -> Type) -> Type}.
-    (* Context `{As : (@type T -> Type) -> Type}. *)
-
-    Fixpoint Typ_0 (form : Type) (ty : type) : Type :=
-    (* Fixpoint Typ_0 (ty : @type T) : Type := *)
-      match ty with
-      | baseT b => b
-      | formulaT => form
-      (* | prodT ty1 ty2 => prod (Typ_0 ty1) (Typ_0 ty2) *)
-      (* | sumT ty1 ty2 => sum (Typ_0 ty1) (Typ_0 ty2) *)
-      (* | listT ty' => list (Typ_0 ty') *)
-      | funT ty1 ty2 => (Typ_0 form ty1 -> Typ_0 form ty2)
-      (* | positiveT => positive *)
-      | pgmapT ty' => gmap positive (Typ_0 form ty')
-      (* | gmapTpos ty' => gmap positive (Typ_0 ty') *)
-      (* | @gmapT _ K EqDec Cnt ty' => @gmap K EqDec Cnt (Typ_0 ty') *)
-      end.
-
-    Fixpoint Typ (i : index) : @type -> Type :=
-      Typ_0 (match i with
-             | O => Empty_set
-             | S j => @t (Typ j) (As (Typ j))
-             end).
-
-    (* Fixpoint Typ_0 (ty : @type T) : Type := *)
-    (* (* Fixpoint Typ_0 (ty : @type T) : Type := *) *)
-    (*   match ty with *)
-    (*   | baseT b => TSem b *)
-    (*   | formulaT => unit *)
-    (*   | prodT ty1 ty2 => prod (Typ_0 ty1) (Typ_0 ty2) *)
-    (*   | sumT ty1 ty2 => sum (Typ_0 ty1) (Typ_0 ty2) *)
-    (*   | listT ty' => list (Typ_0 ty') *)
-    (*   | funT ty1 ty2 => (Typ_0 ty1 -> Typ_0 ty2) *)
-    (*   | positiveT => positive *)
-    (*   | gmapTpos ty' => gmap positive (Typ_0 ty') *)
-    (*   (* | @gmapT _ K EqDec Cnt ty' => @gmap K EqDec Cnt (Typ_0 ty') *) *)
-    (*   end. *)
-
-    (* Fixpoint Typ (i : index) : @type T -> Type := *)
-    (*   match i with *)
-    (*   | O => Typ_0 *)
-    (*   | S j => *)
-    (*       fix Typ_aux (ty : @type T) : Type := *)
-    (*     match ty with *)
-    (*     | baseT b => TSem b *)
-    (*     | formulaT => @t T (Typ j) (As (Typ j)) *)
-    (*     | prodT ty1 ty2 => prod (Typ_aux ty1) (Typ_aux ty2) *)
-    (*     | sumT ty1 ty2 => sum (Typ_aux ty1) (Typ_aux ty2) *)
-    (*     | listT ty' => list (Typ_aux ty') *)
-    (*     | funT ty1 ty2 => (Typ_aux ty1 -> Typ_aux ty2) *)
-    (*     | positiveT => positive *)
-    (*     | gmapTpos ty' => gmap positive (Typ_aux ty') *)
-    (*     (* | @gmapT _ K EqDec Cnt ty' => @gmap K EqDec Cnt (Typ_aux ty') *) *)
-    (*     end *)
-    (*   end. *)
-
-  End INTERP_TYPE.
-
-  Section INTERP.
-
-    Context `{Σ : GRA.t}.
-    (* Context `{T : Type}. *)
-    (* Context `{TSem : T -> Type}. *)
-    Context `{As : (type -> Type) -> Type}.
-    (* Context `{As : (@type T -> Type) -> Type}. *)
-
-    Local Notation typing := (@Typ As).
-    (* Local Notation typing := (@Typ T TSem As). *)
-
-    Context `{interp_atoms : forall (n : index), As (typing n) -> iProp}.
-    (* Context `{Atoms : @IInvSet Σ (fun (n : index) => As (typing n))}. *)
-
-    Fixpoint to_semantics_0
-             n (sem : (typing n formulaT) -> iProp) (syn : @t (typing n) (As (typing n)))
-      : iProp :=
-      match syn with
-      | atom a => interp_atoms n a
-      | lift u => sem u
-      | sepconj p q => Sepconj (to_semantics_0 n sem p) (to_semantics_0 n sem q)
-      | pure P => Pure P
-      | univ ty p => Univ (fun (x : typing n ty) => to_semantics_0 n sem (p x))
-      | ex ty p => Ex (fun (x : typing n ty) => to_semantics_0 n sem (p x))
-      | and p q => And (to_semantics_0 n sem p) (to_semantics_0 n sem q)
-      | or p q => Or (to_semantics_0 n sem p) (to_semantics_0 n sem q)
-      | impl p q => Impl (to_semantics_0 n sem p) (to_semantics_0 n sem q)
-      | wand p q => Wand (to_semantics_0 n sem p) (to_semantics_0 n sem q)
-      | empty => Emp
-      | persistently p => Persistently (to_semantics_0 n sem p)
-      | plainly p => IProp.Plainly (to_semantics_0 n sem p)
-      | upd p => Upd (to_semantics_0 n sem p)
-      end.
-
-    Let cast_typing n : typing (S n) formulaT -> @t (typing n) (As (typing n)) :=
-      fun p => p.
-
-    Fixpoint to_semantics n : @t (typing n) (As (typing n)) -> iProp :=
-      to_semantics_0 n (match n with
-                        | O => fun _ => ⌜False⌝%I
-                        | S m => fun (p : typing (S m) formulaT) => to_semantics m (cast_typing m p)
-                        end).
-
-    (* Fixpoint to_semantics_0 (syn : @t T (typing O) (As (typing O))) : iProp := *)
-    (*   match syn with *)
-    (*   | atom a => interp_atoms O a *)
-    (*   (* | atom a => prop O a *) *)
-    (*   | lift u => ⌜False⌝%I *)
-    (*   (* | lower u => (fun (x : unit) => ⌜False⌝%I) u *) *)
-    (*   | sepconj p q => Sepconj (to_semantics_0 p) (to_semantics_0 q) *)
-    (*   | pure P => Pure P *)
-    (*   | univ ty p => Univ (fun (x : typing O ty) => to_semantics_0 (p x)) *)
-    (*   | ex ty p => Ex (fun (x : typing O ty) => to_semantics_0 (p x)) *)
-    (*   | and p q => And (to_semantics_0 p) (to_semantics_0 q) *)
-    (*   | or p q => Or (to_semantics_0 p) (to_semantics_0 q) *)
-    (*   | impl p q => Impl (to_semantics_0 p) (to_semantics_0 q) *)
-    (*   | wand p q => Wand (to_semantics_0 p) (to_semantics_0 q) *)
-    (*   | empty => Emp *)
-    (*   | persistently p => Persistently (to_semantics_0 p) *)
-    (*   | plainly p => IProp.Plainly (to_semantics_0 p) *)
-    (*   | upd p => Upd (to_semantics_0 p) *)
-    (*   end. *)
-
-    (* Fixpoint to_semantics (i : index) : @t T (typing i) (As (typing i)) -> iProp := *)
-    (*   match i with *)
-    (*   | O => to_semantics_0 *)
-    (*   | S j => *)
-    (*       fix to_semantics_aux (syn : @t T (typing (S j)) (As (typing (S j)))) : iProp := *)
-    (*     match syn with *)
-    (*     | atom a => interp_atoms (S j) a *)
-    (*     (* | atom a => prop (S j) a *) *)
-    (*     | lift syn' => to_semantics j syn' *)
-    (*     | sepconj p q => Sepconj (to_semantics_aux p) (to_semantics_aux q) *)
-    (*     | pure P => Pure P *)
-    (*     | univ ty p => Univ (fun (x : typing (S j) ty) => to_semantics_aux (p x)) *)
-    (*     | ex ty p => Ex (fun (x : typing (S j) ty) => to_semantics_aux (p x)) *)
-    (*     | and p q => And (to_semantics_aux p) (to_semantics_aux q) *)
-    (*     | or p q => Or (to_semantics_aux p) (to_semantics_aux q) *)
-    (*     | impl p q => Impl (to_semantics_aux p) (to_semantics_aux q) *)
-    (*     | wand p q => Wand (to_semantics_aux p) (to_semantics_aux q) *)
-    (*     | empty => Emp *)
-    (*     | persistently p => Persistently (to_semantics_aux p) *)
-    (*     | plainly p => IProp.Plainly (to_semantics_aux p) *)
-    (*     | upd p => Upd (to_semantics_aux p) *)
-    (*     end *)
-    (*   end. *)
-
-  End INTERP.
-
-  Section INDEXED_INVSET.
-
-    Context `{Σ : GRA.t}.
-    (* Context `{T : Type}. *)
-    (* Context `{TSem : T -> Type}. *)
-    Context `{As : (type -> Type) -> Type}.
-    (* Context `{As : (@type T -> Type) -> Type}. *)
-
-    Local Notation typing := (@Typ As).
-    Local Notation Formulas := (fun (i : index) => @t (typing i) (As (typing i))).
-    (* Local Notation typing := (@Typ T TSem As). *)
-    (* Local Notation Formulas := (fun (i : index) => @t T (typing i) (As (typing i))). *)
-
-    Context `{interp_atoms : forall (n : index), As (typing n) -> iProp}.
-    (* Context `{Atoms : @IInvSet Σ (fun (n : index) => As (typing n))}. *)
-
-    Global Instance IISet : @IInvSet Σ Formulas :=
-      {| prop := @to_semantics Σ As interp_atoms |}.
-      (* {| prop := @to_semantics Σ T TSem As interp_atoms |}. *)
-      (* {| prop := @to_semantics Σ T TSem As Atoms |}. *)
-
-  End INDEXED_INVSET.
-
-  Section INV_IN.
-
-    Context `{Σ : GRA.t}.
-    Context `{As : (type -> Type) -> Type}.
-    (* Context `{T : Type}. *)
-    (* Context `{TSem : T -> Type}. *)
-    (* Context `{As : (@type T -> Type) -> Type}. *)
-
-    Local Notation typing := (@Typ As).
-    Local Notation Formulas := (fun (i : index) => @t (typing i) (As (typing i))).
-    (* Local Notation typing := (@Typ T TSem As). *)
-    (* Local Notation Formulas := (fun (i : index) => @t T (typing i) (As (typing i))). *)
-
-    Context `{interp_atoms : forall (n : index), As (typing n) -> iProp}.
-    (* Context `{Atoms : @IInvSet Σ (fun (n : index) => As (typing n))}. *)
-
-    Global Program Instance IIIn (i : index) (p : Formulas i)
-      : @IInvIn Σ Formulas (IISet (interp_atoms:=interp_atoms)) i (@to_semantics Σ As interp_atoms i p) :=
-      (* : @IInvIn Σ Formulas IISet i (@to_semantics Σ T TSem As Atoms i p) := *)
-      { inhabitant := p }.
-    Next Obligation.
-      intros. simpl in *. done.
-    Qed.
-
-    (* Global Program Instance IIIn (i : index) (p : Formulas i) *)
-    (*   : @IInvIn Σ Formulas (IISet (interp_atoms:=interp_atoms)) i (@to_semantics Σ T TSem As interp_atoms i p) := *)
-    (*   (* : @IInvIn Σ Formulas IISet i (@to_semantics Σ T TSem As Atoms i p) := *) *)
-    (*   { inhabitant := p }. *)
-    (* Next Obligation. *)
-    (*   intros. simpl in *. done. *)
-    (* Qed. *)
-
-  End INV_IN.
-
-  Section RED.
-
-    Context `{Σ : GRA.t}.
-    Context `{As : (type -> Type) -> Type}.
-    (* Context `{T : Type}. *)
-    (* Context `{TSem : T -> Type}. *)
-    (* Context `{As : (@type T -> Type) -> Type}. *)
-
-    Local Notation typing := (@Typ As).
-    Local Notation Formulas := (fun (i : index) => @t (typing i) (As (typing i))).
-    (* Local Notation typing := (@Typ T TSem As). *)
-    (* Local Notation Formulas := (fun (i : index) => @t T (typing i) (As (typing i))). *)
-
-    Context `{interp_atoms : forall (n : index), As (typing n) -> iProp}.
-
-    Local Notation Sem := (fun i p => @to_semantics Σ As interp_atoms i p).
-    (* Local Notation Sem := (fun i p => @to_semantics Σ T TSem As interp_atoms i p). *)
-
-    Lemma to_semantics_empty
-          n
-      :
-      Sem n empty = emp%I.
-    Proof.
-      induction n; ss.
-    Qed.
-
-    Lemma to_semantics_red_sepconj
-          n p q
-      :
-      Sem n (sepconj p q) = ((Sem n p) ∗ (Sem n q))%I.
-    Proof.
-      induction n; ss.
-    Qed.
-
-    Lemma to_semantics_red_or
-          n p q
-      :
-      Sem n (or p q) = ((Sem n p) ∨ (Sem n q))%I.
-    Proof.
-      induction n; ss.
-    Qed.
-
-    Lemma to_semantics_red_atom
-          n a
-      :
-      Sem n (atom a) = interp_atoms n a.
-    Proof.
-      induction n; ss.
-    Qed.
-
-    Lemma to_semantics_red_ex
-          n ty f
-      :
-      Sem n (ex ty f) = (∃ (x : typing n ty), Sem n (f x))%I.
-    Proof.
-      induction n; ss.
-    Qed.
-
-    Lemma to_semantics_red_lift
-          n p
-      :
-      Sem (S n) (lift p) = Sem n p.
-    Proof.
-      ss.
-    Qed.
-
-  End RED.
-
-  Section GMAP.
-
-    Context `{Σ : GRA.t}.
-    Context `{As : (type -> Type) -> Type}.
-
-    Local Notation typing := (@Typ As).
-    Local Notation Formulas := (fun (i : index) => @t (typing i) (As (typing i))).
-
-    Context `{interp_atoms : forall (n : index), As (typing n) -> iProp}.
-
-    (* Maybe we can make Syntax as an instance of bi. *)
-    Definition star_gmap
-               (n : index) (I : typing (S n) (pgmapT formulaT))
-               (f : positive -> Formulas n -> Formulas n)
-      : Formulas n :=
-      fold_right (fun hd tl => @sepconj (typing n) (As (typing n)) (uncurry f hd) tl) empty (map_to_list I).
-
-
-    Local Notation Sem := (fun i p => @to_semantics Σ As interp_atoms i p).
-
-    Lemma star_gmap_iProp
-          n I f
-      :
-      Sem n (star_gmap n I f) =
-        ([∗ map] i ↦ p ∈ I, Sem n (f i p))%I.
-    Proof.
-      ss. unfold big_opM. rewrite seal_eq. unfold big_op.big_opM_def.
-      unfold star_gmap. ss. remember (map_to_list I) as L.
-      clear HeqL I. induction L.
-      { ss. apply to_semantics_empty. }
-      ss. rewrite to_semantics_red_sepconj. rewrite IHL. f_equal.
-      destruct a. ss.
-    Qed.
-
-  End GMAP.
-
-End Syntax.
+(*     Lemma star_gmap_iProp *)
+(*           n I f *)
+(*       : *)
+(*       Sem n (star_gmap n I f) = *)
+(*         ([∗ map] i ↦ p ∈ I, Sem n (f i p))%I. *)
+(*     Proof. *)
+(*       ss. unfold big_opM. rewrite seal_eq. unfold big_op.big_opM_def. *)
+(*       unfold star_gmap. ss. remember (map_to_list I) as L. *)
+(*       clear HeqL I. induction L. *)
+(*       { ss. apply to_semantics_empty. } *)
+(*       ss. rewrite to_semantics_red_sepconj. rewrite IHL. f_equal. *)
+(*       destruct a. ss. *)
+(*     Qed. *)
+
+(*   End GMAP. *)
+
+
+
+
+
+
+
+
+
+
+(* (* Old version *) *)
+(* Module Syntax. *)
+
+(*   Local Notation index := nat. *)
+
+(*   Section TYPE. *)
+
+(*     (* Context `{T : Type}. *) *)
+
+(*     Inductive type : Type := *)
+(*     | baseT (t : Type) : type *)
+(*     (* | baseT (t : T) : type *) *)
+(*     | formulaT : type *)
+(*     (* | prodT : type -> type -> type *) *)
+(*     (* | sumT : type -> type -> type *) *)
+(*     (* | listT : type -> type *) *)
+(*     | funT : type -> type -> type *)
+(*     (* | positiveT : type *) *)
+(*     | pgmapT : type -> type. *)
+(*     (* | gmapT (K : Type) {EqDec : EqDecision K} {Cnt : Countable K} : type -> type. *) *)
+
+(*   (* If we define for a general gmapT with EqDec and Countable, *)
+(*       universe inconsistency when checking (in TemporalLogic.Atoms) *)
+(*       ========== *)
+(*       Context `{Σ : GRA.t}. *)
+(*       Context `{T : Type}. *)
+(*       Context `{TSem : T -> Type}. *)
+(*       Local Notation typing := (@Syntax.Typ T TSem (@t T)). *)
+(*       Local Notation As := (fun (i : index) => @t T (typing i)). *)
+
+(*       Context `{@GRA.inG (IInvSetRA As) Σ}. *)
+(*       ========== *)
+(*       with an error message *)
+(*       ========== *)
+(*       The term "t" has type *)
+(*       "Type@{max(Set+1,Fairness.LogicSyntaxHOAS.59,Syntax.type.u0+1,Fairness.LogicSyntaxHOAS.64,Fairness.LogicSyntaxHOAS.65,RelDecision.u0,RelDecision.u1)}" *)
+(*       while it is expected to have type "Type@{IInvSetRA.u0}" (universe inconsistency: Cannot enforce *)
+(*       Fairness.LogicSyntaxHOAS.64 <= IInvSetRA.u0 because IInvSetRA.u0 <= InvSetRA.u0 *)
+(*       <= URA.agree_obligation_4.u0 <= URA.t.u0 < MRet.u0 = Fairness.LogicSyntaxHOAS.64). *)
+(*       ========== *)
+(*       Seems like there is a strict order between URA.t and MRet, *)
+(*       and either EqDec or Countable uses MRet. *)
+(*       ========== *)
+(*       Found out that PCM.GRA.of_list introduces URA.t.u0 = RA.t.u0 < MRet.u0. *)
+(*    *) *)
+
+(*   End TYPE. *)
+
+(*   Section SYNTAX. *)
+
+(*     (* Context `{T : Type}. *) *)
+(*     Context `{Typ : type -> Type}. *)
+(*     (* Context `{Typ : @type T -> Type}. *) *)
+(*     Context `{A : Type}. *)
+
+(*     Inductive t : Type := *)
+(*       atom (a : A) : t *)
+(*     | lift : (Typ formulaT) -> t *)
+(*     | sepconj (p q : t) : t *)
+(*     | pure (P : Prop) : t *)
+(*     | univ : forall ty, (Typ ty -> t) -> t *)
+(*     | ex : forall ty, (Typ ty -> t) -> t *)
+(*     | and (p q : t) : t *)
+(*     | or (p q : t) : t *)
+(*     | impl (p q : t) : t *)
+(*     | wand (p q : t) : t *)
+(*     | empty : t *)
+(*     | persistently (p : t) : t *)
+(*     | plainly (p : t) : t *)
+(*     | upd (p : t) : t *)
+(*     . *)
+
+(*   End SYNTAX. *)
+
+(*   Section INTERP_TYPE. *)
+
+(*     (* Context `{T : Type}. *) *)
+(*     (* Context `{TSem : T -> Type}. *) *)
+(*     Context `{As : (type -> Type) -> Type}. *)
+(*     (* Context `{As : (@type T -> Type) -> Type}. *) *)
+
+(*     Fixpoint Typ_0 (form : Type) (ty : type) : Type := *)
+(*     (* Fixpoint Typ_0 (ty : @type T) : Type := *) *)
+(*       match ty with *)
+(*       | baseT b => b *)
+(*       | formulaT => form *)
+(*       (* | prodT ty1 ty2 => prod (Typ_0 ty1) (Typ_0 ty2) *) *)
+(*       (* | sumT ty1 ty2 => sum (Typ_0 ty1) (Typ_0 ty2) *) *)
+(*       (* | listT ty' => list (Typ_0 ty') *) *)
+(*       | funT ty1 ty2 => (Typ_0 form ty1 -> Typ_0 form ty2) *)
+(*       (* | positiveT => positive *) *)
+(*       | pgmapT ty' => gmap positive (Typ_0 form ty') *)
+(*       (* | gmapTpos ty' => gmap positive (Typ_0 ty') *) *)
+(*       (* | @gmapT _ K EqDec Cnt ty' => @gmap K EqDec Cnt (Typ_0 ty') *) *)
+(*       end. *)
+
+(*     Fixpoint Typ (i : index) : @type -> Type := *)
+(*       Typ_0 (match i with *)
+(*              | O => Empty_set *)
+(*              | S j => @t (Typ j) (As (Typ j)) *)
+(*              end). *)
+
+(*     (* Fixpoint Typ_0 (ty : @type T) : Type := *) *)
+(*     (* (* Fixpoint Typ_0 (ty : @type T) : Type := *) *) *)
+(*     (*   match ty with *) *)
+(*     (*   | baseT b => TSem b *) *)
+(*     (*   | formulaT => unit *) *)
+(*     (*   | prodT ty1 ty2 => prod (Typ_0 ty1) (Typ_0 ty2) *) *)
+(*     (*   | sumT ty1 ty2 => sum (Typ_0 ty1) (Typ_0 ty2) *) *)
+(*     (*   | listT ty' => list (Typ_0 ty') *) *)
+(*     (*   | funT ty1 ty2 => (Typ_0 ty1 -> Typ_0 ty2) *) *)
+(*     (*   | positiveT => positive *) *)
+(*     (*   | gmapTpos ty' => gmap positive (Typ_0 ty') *) *)
+(*     (*   (* | @gmapT _ K EqDec Cnt ty' => @gmap K EqDec Cnt (Typ_0 ty') *) *) *)
+(*     (*   end. *) *)
+
+(*     (* Fixpoint Typ (i : index) : @type T -> Type := *) *)
+(*     (*   match i with *) *)
+(*     (*   | O => Typ_0 *) *)
+(*     (*   | S j => *) *)
+(*     (*       fix Typ_aux (ty : @type T) : Type := *) *)
+(*     (*     match ty with *) *)
+(*     (*     | baseT b => TSem b *) *)
+(*     (*     | formulaT => @t T (Typ j) (As (Typ j)) *) *)
+(*     (*     | prodT ty1 ty2 => prod (Typ_aux ty1) (Typ_aux ty2) *) *)
+(*     (*     | sumT ty1 ty2 => sum (Typ_aux ty1) (Typ_aux ty2) *) *)
+(*     (*     | listT ty' => list (Typ_aux ty') *) *)
+(*     (*     | funT ty1 ty2 => (Typ_aux ty1 -> Typ_aux ty2) *) *)
+(*     (*     | positiveT => positive *) *)
+(*     (*     | gmapTpos ty' => gmap positive (Typ_aux ty') *) *)
+(*     (*     (* | @gmapT _ K EqDec Cnt ty' => @gmap K EqDec Cnt (Typ_aux ty') *) *) *)
+(*     (*     end *) *)
+(*     (*   end. *) *)
+
+(*   End INTERP_TYPE. *)
+
+(*   Section INTERP. *)
+
+(*     Context `{Σ : GRA.t}. *)
+(*     (* Context `{T : Type}. *) *)
+(*     (* Context `{TSem : T -> Type}. *) *)
+(*     Context `{As : (type -> Type) -> Type}. *)
+(*     (* Context `{As : (@type T -> Type) -> Type}. *) *)
+
+(*     Local Notation typing := (@Typ As). *)
+(*     (* Local Notation typing := (@Typ T TSem As). *) *)
+
+(*     Context `{interp_atoms : forall (n : index), As (typing n) -> iProp}. *)
+(*     (* Context `{Atoms : @IInvSet Σ (fun (n : index) => As (typing n))}. *) *)
+
+(*     Fixpoint to_semantics_0 *)
+(*              n (sem : (typing n formulaT) -> iProp) (syn : @t (typing n) (As (typing n))) *)
+(*       : iProp := *)
+(*       match syn with *)
+(*       | atom a => interp_atoms n a *)
+(*       | lift u => sem u *)
+(*       | sepconj p q => Sepconj (to_semantics_0 n sem p) (to_semantics_0 n sem q) *)
+(*       | pure P => Pure P *)
+(*       | univ ty p => Univ (fun (x : typing n ty) => to_semantics_0 n sem (p x)) *)
+(*       | ex ty p => Ex (fun (x : typing n ty) => to_semantics_0 n sem (p x)) *)
+(*       | and p q => And (to_semantics_0 n sem p) (to_semantics_0 n sem q) *)
+(*       | or p q => Or (to_semantics_0 n sem p) (to_semantics_0 n sem q) *)
+(*       | impl p q => Impl (to_semantics_0 n sem p) (to_semantics_0 n sem q) *)
+(*       | wand p q => Wand (to_semantics_0 n sem p) (to_semantics_0 n sem q) *)
+(*       | empty => Emp *)
+(*       | persistently p => Persistently (to_semantics_0 n sem p) *)
+(*       | plainly p => IProp.Plainly (to_semantics_0 n sem p) *)
+(*       | upd p => Upd (to_semantics_0 n sem p) *)
+(*       end. *)
+
+(*     Let cast_typing n : typing (S n) formulaT -> @t (typing n) (As (typing n)) := *)
+(*       fun p => p. *)
+
+(*     Fixpoint to_semantics n : @t (typing n) (As (typing n)) -> iProp := *)
+(*       to_semantics_0 n (match n with *)
+(*                         | O => fun _ => ⌜False⌝%I *)
+(*                         | S m => fun (p : typing (S m) formulaT) => to_semantics m (cast_typing m p) *)
+(*                         end). *)
+
+(*     (* Fixpoint to_semantics_0 (syn : @t T (typing O) (As (typing O))) : iProp := *) *)
+(*     (*   match syn with *) *)
+(*     (*   | atom a => interp_atoms O a *) *)
+(*     (*   (* | atom a => prop O a *) *) *)
+(*     (*   | lift u => ⌜False⌝%I *) *)
+(*     (*   (* | lower u => (fun (x : unit) => ⌜False⌝%I) u *) *) *)
+(*     (*   | sepconj p q => Sepconj (to_semantics_0 p) (to_semantics_0 q) *) *)
+(*     (*   | pure P => Pure P *) *)
+(*     (*   | univ ty p => Univ (fun (x : typing O ty) => to_semantics_0 (p x)) *) *)
+(*     (*   | ex ty p => Ex (fun (x : typing O ty) => to_semantics_0 (p x)) *) *)
+(*     (*   | and p q => And (to_semantics_0 p) (to_semantics_0 q) *) *)
+(*     (*   | or p q => Or (to_semantics_0 p) (to_semantics_0 q) *) *)
+(*     (*   | impl p q => Impl (to_semantics_0 p) (to_semantics_0 q) *) *)
+(*     (*   | wand p q => Wand (to_semantics_0 p) (to_semantics_0 q) *) *)
+(*     (*   | empty => Emp *) *)
+(*     (*   | persistently p => Persistently (to_semantics_0 p) *) *)
+(*     (*   | plainly p => IProp.Plainly (to_semantics_0 p) *) *)
+(*     (*   | upd p => Upd (to_semantics_0 p) *) *)
+(*     (*   end. *) *)
+
+(*     (* Fixpoint to_semantics (i : index) : @t T (typing i) (As (typing i)) -> iProp := *) *)
+(*     (*   match i with *) *)
+(*     (*   | O => to_semantics_0 *) *)
+(*     (*   | S j => *) *)
+(*     (*       fix to_semantics_aux (syn : @t T (typing (S j)) (As (typing (S j)))) : iProp := *) *)
+(*     (*     match syn with *) *)
+(*     (*     | atom a => interp_atoms (S j) a *) *)
+(*     (*     (* | atom a => prop (S j) a *) *) *)
+(*     (*     | lift syn' => to_semantics j syn' *) *)
+(*     (*     | sepconj p q => Sepconj (to_semantics_aux p) (to_semantics_aux q) *) *)
+(*     (*     | pure P => Pure P *) *)
+(*     (*     | univ ty p => Univ (fun (x : typing (S j) ty) => to_semantics_aux (p x)) *) *)
+(*     (*     | ex ty p => Ex (fun (x : typing (S j) ty) => to_semantics_aux (p x)) *) *)
+(*     (*     | and p q => And (to_semantics_aux p) (to_semantics_aux q) *) *)
+(*     (*     | or p q => Or (to_semantics_aux p) (to_semantics_aux q) *) *)
+(*     (*     | impl p q => Impl (to_semantics_aux p) (to_semantics_aux q) *) *)
+(*     (*     | wand p q => Wand (to_semantics_aux p) (to_semantics_aux q) *) *)
+(*     (*     | empty => Emp *) *)
+(*     (*     | persistently p => Persistently (to_semantics_aux p) *) *)
+(*     (*     | plainly p => IProp.Plainly (to_semantics_aux p) *) *)
+(*     (*     | upd p => Upd (to_semantics_aux p) *) *)
+(*     (*     end *) *)
+(*     (*   end. *) *)
+
+(*   End INTERP. *)
+
+(*   Section INDEXED_INVSET. *)
+
+(*     Context `{Σ : GRA.t}. *)
+(*     (* Context `{T : Type}. *) *)
+(*     (* Context `{TSem : T -> Type}. *) *)
+(*     Context `{As : (type -> Type) -> Type}. *)
+(*     (* Context `{As : (@type T -> Type) -> Type}. *) *)
+
+(*     Local Notation typing := (@Typ As). *)
+(*     Local Notation Formulas := (fun (i : index) => @t (typing i) (As (typing i))). *)
+(*     (* Local Notation typing := (@Typ T TSem As). *) *)
+(*     (* Local Notation Formulas := (fun (i : index) => @t T (typing i) (As (typing i))). *) *)
+
+(*     Context `{interp_atoms : forall (n : index), As (typing n) -> iProp}. *)
+(*     (* Context `{Atoms : @IInvSet Σ (fun (n : index) => As (typing n))}. *) *)
+
+(*     Global Instance IISet : @IInvSet Σ Formulas := *)
+(*       {| prop := @to_semantics Σ As interp_atoms |}. *)
+(*       (* {| prop := @to_semantics Σ T TSem As interp_atoms |}. *) *)
+(*       (* {| prop := @to_semantics Σ T TSem As Atoms |}. *) *)
+
+(*   End INDEXED_INVSET. *)
+
+(*   Section INV_IN. *)
+
+(*     Context `{Σ : GRA.t}. *)
+(*     Context `{As : (type -> Type) -> Type}. *)
+(*     (* Context `{T : Type}. *) *)
+(*     (* Context `{TSem : T -> Type}. *) *)
+(*     (* Context `{As : (@type T -> Type) -> Type}. *) *)
+
+(*     Local Notation typing := (@Typ As). *)
+(*     Local Notation Formulas := (fun (i : index) => @t (typing i) (As (typing i))). *)
+(*     (* Local Notation typing := (@Typ T TSem As). *) *)
+(*     (* Local Notation Formulas := (fun (i : index) => @t T (typing i) (As (typing i))). *) *)
+
+(*     Context `{interp_atoms : forall (n : index), As (typing n) -> iProp}. *)
+(*     (* Context `{Atoms : @IInvSet Σ (fun (n : index) => As (typing n))}. *) *)
+
+(*     Global Program Instance IIIn (i : index) (p : Formulas i) *)
+(*       : @IInvIn Σ Formulas (IISet (interp_atoms:=interp_atoms)) i (@to_semantics Σ As interp_atoms i p) := *)
+(*       (* : @IInvIn Σ Formulas IISet i (@to_semantics Σ T TSem As Atoms i p) := *) *)
+(*       { inhabitant := p }. *)
+(*     Next Obligation. *)
+(*       intros. simpl in *. done. *)
+(*     Qed. *)
+
+(*     (* Global Program Instance IIIn (i : index) (p : Formulas i) *) *)
+(*     (*   : @IInvIn Σ Formulas (IISet (interp_atoms:=interp_atoms)) i (@to_semantics Σ T TSem As interp_atoms i p) := *) *)
+(*     (*   (* : @IInvIn Σ Formulas IISet i (@to_semantics Σ T TSem As Atoms i p) := *) *) *)
+(*     (*   { inhabitant := p }. *) *)
+(*     (* Next Obligation. *) *)
+(*     (*   intros. simpl in *. done. *) *)
+(*     (* Qed. *) *)
+
+(*   End INV_IN. *)
+
+(*   Section RED. *)
+
+(*     Context `{Σ : GRA.t}. *)
+(*     Context `{As : (type -> Type) -> Type}. *)
+(*     (* Context `{T : Type}. *) *)
+(*     (* Context `{TSem : T -> Type}. *) *)
+(*     (* Context `{As : (@type T -> Type) -> Type}. *) *)
+
+(*     Local Notation typing := (@Typ As). *)
+(*     Local Notation Formulas := (fun (i : index) => @t (typing i) (As (typing i))). *)
+(*     (* Local Notation typing := (@Typ T TSem As). *) *)
+(*     (* Local Notation Formulas := (fun (i : index) => @t T (typing i) (As (typing i))). *) *)
+
+(*     Context `{interp_atoms : forall (n : index), As (typing n) -> iProp}. *)
+
+(*     Local Notation Sem := (fun i p => @to_semantics Σ As interp_atoms i p). *)
+(*     (* Local Notation Sem := (fun i p => @to_semantics Σ T TSem As interp_atoms i p). *) *)
+
+(*     Lemma to_semantics_empty *)
+(*           n *)
+(*       : *)
+(*       Sem n empty = emp%I. *)
+(*     Proof. *)
+(*       induction n; ss. *)
+(*     Qed. *)
+
+(*     Lemma to_semantics_red_sepconj *)
+(*           n p q *)
+(*       : *)
+(*       Sem n (sepconj p q) = ((Sem n p) ∗ (Sem n q))%I. *)
+(*     Proof. *)
+(*       induction n; ss. *)
+(*     Qed. *)
+
+(*     Lemma to_semantics_red_or *)
+(*           n p q *)
+(*       : *)
+(*       Sem n (or p q) = ((Sem n p) ∨ (Sem n q))%I. *)
+(*     Proof. *)
+(*       induction n; ss. *)
+(*     Qed. *)
+
+(*     Lemma to_semantics_red_atom *)
+(*           n a *)
+(*       : *)
+(*       Sem n (atom a) = interp_atoms n a. *)
+(*     Proof. *)
+(*       induction n; ss. *)
+(*     Qed. *)
+
+(*     Lemma to_semantics_red_ex *)
+(*           n ty f *)
+(*       : *)
+(*       Sem n (ex ty f) = (∃ (x : typing n ty), Sem n (f x))%I. *)
+(*     Proof. *)
+(*       induction n; ss. *)
+(*     Qed. *)
+
+(*     Lemma to_semantics_red_lift *)
+(*           n p *)
+(*       : *)
+(*       Sem (S n) (lift p) = Sem n p. *)
+(*     Proof. *)
+(*       ss. *)
+(*     Qed. *)
+
+(*   End RED. *)
+
+(*   Section GMAP. *)
+
+(*     Context `{Σ : GRA.t}. *)
+(*     Context `{As : (type -> Type) -> Type}. *)
+
+(*     Local Notation typing := (@Typ As). *)
+(*     Local Notation Formulas := (fun (i : index) => @t (typing i) (As (typing i))). *)
+
+(*     Context `{interp_atoms : forall (n : index), As (typing n) -> iProp}. *)
+
+(*     (* Maybe we can make Syntax as an instance of bi. *) *)
+(*     Definition star_gmap *)
+(*                (n : index) (I : typing (S n) (pgmapT formulaT)) *)
+(*                (f : positive -> Formulas n -> Formulas n) *)
+(*       : Formulas n := *)
+(*       fold_right (fun hd tl => @sepconj (typing n) (As (typing n)) (uncurry f hd) tl) empty (map_to_list I). *)
+
+
+(*     Local Notation Sem := (fun i p => @to_semantics Σ As interp_atoms i p). *)
+
+(*     Lemma star_gmap_iProp *)
+(*           n I f *)
+(*       : *)
+(*       Sem n (star_gmap n I f) = *)
+(*         ([∗ map] i ↦ p ∈ I, Sem n (f i p))%I. *)
+(*     Proof. *)
+(*       ss. unfold big_opM. rewrite seal_eq. unfold big_op.big_opM_def. *)
+(*       unfold star_gmap. ss. remember (map_to_list I) as L. *)
+(*       clear HeqL I. induction L. *)
+(*       { ss. apply to_semantics_empty. } *)
+(*       ss. rewrite to_semantics_red_sepconj. rewrite IHL. f_equal. *)
+(*       destruct a. ss. *)
+(*     Qed. *)
+
+(*   End GMAP. *)
+
+(* End Syntax. *)
